wip: verifying simple queue

lawyer/nonblocking/examples/simple_queue.v
@@ -21,16 +21,103 @@ Section MaxExact.
   Definition me_exact (n: nat): iProp Σ. Admitted. 
   Definition me_lb (n: nat): iProp Σ. Admitted. 
 
-End MaxExact. 
+End MaxExact.
 
 
-Class QueueG := {
+Section ListToIMap.
+  Context {A: Type}.
+
+  (* TODO: rename *)
+  Definition list_to_imap: list A -> gmap nat A :=
+    list_to_map ∘ imap pair.
+
+  (* Lemma list_to_imap_spec l: *)
+  (*   forall i, l !! i = list_to_imap l !! i.  *)
+  (* Proof using. *)
+  (*   induction l. *)
+  (*   { set_solver. } *)
+  (*   intros. simpl. *)
+  (*   rewrite lookup_cons. rewrite /list_to_imap. simpl. *)
+  (*   destruct i. *)
+  (*   { by rewrite lookup_insert. } *)
+  (*   rewrite lookup_insert_ne; [| done]. *)
+
+  Local Lemma helper (l: list A) i k:
+    l !! i = (list_to_map (imap (pair ∘ (plus k)) l): gmap nat A) !! (k + i).
+  Proof using.
+    generalize dependent i. generalize dependent k.
+    induction l.
+    { set_solver. }
+    intros. simpl. destruct i.
+    { simpl. by rewrite lookup_insert. }
+    simpl. rewrite lookup_insert_ne; [| lia].
+    rewrite -Nat.add_succ_comm. 
+    erewrite IHl. do 2 f_equal. 
+    apply imap_ext. simpl. intros. f_equal. lia.
+  Qed.
+
+  Lemma list_to_imap_spec l:
+    forall i, list_to_imap l !! i = l !! i.
+  Proof using.
+    intros. rewrite /list_to_imap /compose.
+    symmetry. by rewrite (helper _ _ 0).
+  Qed.
+
+  Lemma list_to_imap_dom l:
+    dom (list_to_imap l) = set_seq 0 (length l).
+  Proof using.
+    apply set_eq. intros i.
+    rewrite elem_of_set_seq elem_of_dom.
+    rewrite list_to_imap_spec. rewrite lookup_lt_is_Some. lia.
+  Qed.    
+
+End ListToIMap.
+
+
+Section HistQueue.
+
+  Definition Node: Set := val * loc.
+  Definition HistNode: Set := loc * Node. 
+  Definition HistQueue := list HistNode.
+
+  Class HistQueuePreG Σ := {
+      hq_map :: inG Σ (authUR (gmapUR nat (agreeR HistNode)));
+  }.
+  
+  Class HistQueueG Σ := {
+      hq_PreG :: HistQueuePreG Σ;
+      hq_γ__map: gname;
+  }.
+
+  Context `{HistQueueG Σ}. 
+  
+  Definition ith_node (i: nat) (nd: HistNode): iProp Σ :=
+    own hq_γ__map (◯ {[ i := to_agree nd ]}).
+
+  Definition hq_auth (hq: HistQueue): iProp Σ := 
+    own hq_γ__map (● (to_agree <$> (list_to_imap hq): gmapUR nat (agreeR HistNode))) ∗
+    ([∗ list] i ↦ hn ∈ hq, ith_node i hn). 
+
+  Definition hq_auth_get_ith i nd hq
+    (ITH: hq !! i = Some nd):
+  hq_auth hq -∗ ith_node i nd ∗ hq_auth hq.
+  Proof using.
+    iIntros "[AUTH #FRAGS]". iFrame "#∗".
+    rewrite big_sepL_lookup_acc; eauto.
+    by iDestruct "FRAGS" as "[??]".
+  Qed.
+
+End HistQueue.
+
+
+Class QueueG Σ := {
     Head: loc; Tail: loc; BeingRead: loc; 
     FreeLater: loc; OldHeadVal: loc;
     γHead: gname; γTail: gname; γBeingRead: gname; 
     γFreeLater: gname; γOldHeadVal: gname;
 
     γHob: gname;
+    q_hq :: HistQueueG Σ;
 }.
 
 
@@ -66,22 +153,22 @@ Section SimpleQueue.
           (SOME "v")
   .
 
-  Definition Node: Set := val * loc. 
-  Definition HistQueue: Set := list (loc * Node).
-
-  Context (QL: QueueG).  
-  (* Let H := Head. QL. *)
-  (* Let T := Tail QL. *)
-  (* Let BR := BeingRead QL. *)
-  (* Let FL := FreeLater QL. *)
-  (* Let OHV := OldHeadVal QL. *)
-
   Section QueueResources. 
 
     Context {Σ} {hG: heap1GS Σ} {iG: invGS_gen HasNoLc Σ}.
   
-    Definition queue_interp (hq: HistQueue) (h t br fl: nat): iProp Σ.
-    Admitted.
+    Context {QL: QueueG Σ}.
+    (* Let H := Head. QL. *)
+    (* Let T := Tail QL. *)
+    (* Let BR := BeingRead QL. *)
+    (* Let FL := FreeLater QL. *)
+    (* Let OHV := OldHeadVal QL. *)
+
+    Definition queue_interp (hq: HistQueue) (h t br fl: nat): iProp Σ :=
+      (* TODO: add other components *)
+      (∃ (nd: HistNode), ⌜ hq !! h = Some nd ⌝ ∗ Head ↦ #(nd.1)) ∗
+      (∃ (nd: HistNode), ⌜ hq !! t = Some nd ⌝ ∗ Tail ↦ #(nd.1))
+    .
   
     Definition dangle (od: option loc): iProp Σ. Admitted.
   
@@ -108,6 +195,7 @@ Section SimpleQueue.
   
     Definition queue_inv_inner (hq: HistQueue) (h t br fl hob: nat)
       (od: option loc) (ohv: val): iProp Σ :=
+      hq_auth hq ∗ 
       queue_interp hq h t br fl ∗ dangle od ∗ OldHeadVal ↦ ohv ∗
       ⌜ fl <= br <= hob /\ hob <= h /\ (fl < h) ⌝ ∗
       auths h t br fl hob ∗
@@ -126,7 +214,7 @@ Section SimpleQueue.
     (* Definition queue_inv (q: loc): iProp Σ := *)
     Definition queue_inv (q: val): iProp Σ :=
       queue_at q ∗ inv queue_ns 
-        (∃ hq h t br fl hob od ohv, queue_inv_inner hq h t br fl hob   od ohv)
+        (∃ hq h t br fl hob od ohv, queue_inv_inner hq h t br fl hob od ohv)
     .
   
   End QueueResources.
@@ -139,6 +227,7 @@ Section SimpleQueue.
 
   Context {Σ} {OHE: OM_HL_Env OP EM Σ}.
   (* Existing Instance OHE.  *)
+  Context {QL: QueueG Σ}.
 
   Context (d: Degree).
 
@@ -153,14 +242,67 @@ Section SimpleQueue.
     simpl. iIntros (Φ) "(#QAT & PH & CPS) POST". rewrite /loc_head.
     rewrite /queue_at. iDestruct "QAT" as %->.
     pure_steps. by iApply "POST".
-  Qed.    
+  Qed.
+
+  Lemma get_tail_spec l τ π q:
+    {{{ (let _: heap1GS Σ := iem_phys _ EM in queue_at l) ∗
+        th_phase_frag τ π q ∗ cp_mul π d get_loc_fuel }}}
+      loc_tail l @ τ
+    {{{ RET #Tail; th_phase_frag τ π q }}}.
+  Proof using.
+    simpl. iIntros (Φ) "(#QAT & PH & CPS) POST". rewrite /loc_tail.
+    rewrite /queue_at. iDestruct "QAT" as %->.
+    pure_steps.
+    wp_bind (Snd _)%E. pure_steps. 
+    by iApply "POST".
+  Qed.
+
+  Lemma dequeue_token_excl:
+    let _: heap1GS Σ := iem_phys _ EM in 
+    dequeue_token -∗ dequeue_token -∗ False.
+  Proof. Admitted.
+
+  Lemma dequeue_resources_excl h1 fl1 h2 fl2:
+    let _: heap1GS Σ := iem_phys _ EM in 
+    dequeue_resources h1 fl1 -∗ dequeue_resources h2 fl2 -∗ False.
+  Proof. Admitted.
+
+  Lemma access_head hq h t br fl:
+    let _: heap1GS Σ := iem_phys _ EM in
+    hq_auth hq -∗ queue_interp hq h t br fl -∗
+      ∃ nd, ith_node h nd ∗ Head ↦ #nd.1 ∗
+             (Head ↦ #nd.1 -∗ hq_auth hq ∗ queue_interp hq h t br fl).
+  Proof using.
+    simpl. iIntros "HQ QI".
+    rewrite /queue_interp. iDestruct "QI" as "((%nd & %HEAD & BR) & ?)".
+    iFrame "BR".
+    iDestruct (hq_auth_get_ith with "[$]") as "[ITH HQ]"; eauto. iFrame.
+    by iIntros "$".
+  Qed.
+
+  Lemma access_tail hq h t br fl:
+    let _: heap1GS Σ := iem_phys _ EM in
+    hq_auth hq -∗ queue_interp hq h t br fl -∗
+      ∃ nd, ith_node t nd ∗ Tail ↦ #nd.1 ∗
+             (Tail ↦ #nd.1 -∗ hq_auth hq ∗ queue_interp hq h t br fl).
+  Proof using.
+    simpl. iIntros "HQ QI".
+    rewrite /queue_interp. iDestruct "QI" as "(? & (%nd & %TAIL & BR))".
+    iFrame "BR".
+    iDestruct (hq_auth_get_ith with "[$]") as "[ITH HQ]"; eauto. iFrame.
+    by iIntros "$".
+  Qed.
+
+  Lemma dequeue_resources_auth_agree h' fl' h t br fl hob:
+    dequeue_resources h' fl' -∗ auths h t br fl hob -∗ ⌜ h' = h /\ fl' = fl ⌝.
+  Proof using. Admitted. 
 
   Lemma dequeue_spec l (τ: locale heap_lang) (π: Phase) (q: Qp):
     {{{ (let _: heap1GS Σ := iem_phys _ EM in queue_inv l) ∗
         (let _: heap1GS Σ := iem_phys _ EM in dequeue_token) ∗ 
           th_phase_frag τ π q ∗ cp_mul π d 50 }}}
       dequeue l @ τ
-    {{{ v, RET #v; th_phase_frag τ π q }}}.
+    {{{ (v: val), RET v; th_phase_frag τ π q ∗ (let _: heap1GS Σ := iem_phys _ EM in dequeue_token) }}}.
   Proof using.
     simpl. iIntros (Φ) "([#QAT #INV] & TOK & PH & CPS) POST". rewrite /dequeue.
     pure_steps.
@@ -169,6 +311,86 @@ Section SimpleQueue.
     { cbv. lia. } 
     iApply (get_head_spec with "[$QAT $CPS' $PH]").
     iIntros "!> PH".
+
+    wp_bind (! _)%E. 
+    iInv "INV" as "(%hq & %h & %t & %br & %fl & %hob & %od & %ohv & inv)" "CLOS".
+    iEval (rewrite /queue_inv_inner) in "inv".
+    iDestruct "inv" as "(>HQ & >QI & DANGLE & OHV & >%ORDER & AUTHS & >%SAFE_BR & RH & DQ)".
+    
+    iApply sswp_MU_wp; [done| ]. 
+    iDestruct (access_head with "[$] [$]") as "(%ch & #HEADch & HEAD & CLOS')".
+    iApply (wp_load with "[$]"). iIntros "!> HEAD".
+    iDestruct ("CLOS'" with "[$]") as "(HQ & QI)".
+    MU_by_burn_cp. iApply wp_value.
+
+    iDestruct "DQ" as "[DR | TOK']".
+    2: { by iDestruct (dequeue_token_excl with "[$] [$]") as "?". }
+
+    iMod ("CLOS" with "[-POST CPS PH DR]") as "_".
+    { by iFrame. }
+    iModIntro.
+    (* TODO: do we need to keep track of previous values at this point? *)
+    clear t br hob od ohv ORDER SAFE_BR hq.
+
+    wp_bind (Rec _ _ _)%E. pure_steps. 
+    
+    split_cps "CPS" get_loc_fuel.
+    { cbv. lia. } 
+    iApply (get_tail_spec with "[$QAT $CPS' $PH]").
+    iIntros "!> PH".
+
+    wp_bind (! _)%E.
+    iInv "INV" as "(%hq & %h_ & %t & %br & %fl_ & %hob & %od & %ohv & inv)" "CLOS".
+    iEval (rewrite /queue_inv_inner) in "inv".
+    iDestruct "inv" as "(>HQ & >QI & DANGLE & OHV & >%ORDER & AUTHS & >%SAFE_BR & RH & DQ)".
+    iApply sswp_MU_wp; [done| ]. 
+    iDestruct (access_tail with "[$] [$]") as "(%ct & #TAILct & TAIL & CLOS')".
+    iApply (wp_load with "[$]"). iIntros "!> TAIL".
+    iDestruct ("CLOS'" with "[$]") as "(HQ & QI)".
+    MU_by_burn_cp. iApply wp_value.
+    iMod ("CLOS" with "[-POST CPS PH DR]") as "_".
+    { by iFrame. }
+    iModIntro.
+    (* TODO: do we need to keep track of previous values at this point? *)
+    clear h_ fl_ br hob od ohv ORDER SAFE_BR hq.
+
+    wp_bind (_ = _)%E.
+    iApply sswp_MU_wp; [done| ].
+    iApply sswp_pure_step.
+    { destruct ch, ct. simpl. tauto. }
+    MU_by_burn_cp. iApply wp_value.
+
+    destruct bool_decide.
+    {
+      iApply sswp_MU_wp_fupd; [done| ]. 
+      iInv "INV" as "(%hq & %h_ & %t' & %br & %fl_ & %hob & %od & %ohv & inv)" "CLOS".
+      iEval (rewrite /queue_inv_inner) in "inv".
+      iDestruct "inv" as "(>HQ & >QI & DANGLE & OHV & >%ORDER & AUTHS & >%SAFE_BR & RH & DQ)".
+      iModIntro.
+      iApply sswp_pure_step; [done| ].
+      do 2 iNext. MU_by_burn_cp.
+      iDestruct "DQ" as "[DR' | TOK]".
+      { by iDestruct (dequeue_resources_excl with "[$] [$]") as "?". }
+      iDestruct (dequeue_resources_auth_agree with "[$] [$]") as %[-> ->]. 
+      iMod ("CLOS" with "[-POST CPS PH TOK]") as "_".
+      { by iFrame. }
+      iModIntro. pure_steps.
+      iApply "POST". iFrame. }
+
+    (* TODO: can we just forget about the tail from now on? *)
+    iClear "TAILct". clear t ct.
+    pure_steps. 
+
+  
+      pure_steps. iApply 
+      
+      Unset Printing Notations.
+      wp_bind (
+          
+
+
+
+    
 
     
 End SimpleQueue.
